make the predicate generic

Validator/Expr/BCFG.lean
@@ -3,7 +3,6 @@ import Std
 import Validator.Std.Vec
 
 import Validator.Expr.Regex
-import Validator.Expr.Pred
 
 namespace BalancedContextFreeGrammar
 
@@ -11,15 +10,15 @@ abbrev Ref n := Fin n
 
 -- Balanced Context Free Grammars have the restriction that each non-terminal cannot represent any regular expression,
 -- but only regular expressions that are surrounded by a start and end terminal.
-structure Rule (n: Nat) (α: Type) (Φ: (α: Type) -> Type) where
-  enter: Φ α
+structure Rule (n: Nat) (φ: Type) where
+  enter: φ
   child: Regex (Ref n)
-  leave: Φ α
+  leave: φ
 
-abbrev RegexRule (n: Nat) (α: Type) (Φ: (α: Type) -> Type) := Regex ((Φ α) ⊕ (Ref n))
+abbrev RegexRule (n: Nat) (φ: Type) := Regex (φ ⊕ (Ref n))
 
-def Rule.toRegex {n: Nat} {α: Type} {Φ: (α: Type) -> Type}
-  (r: Rule n α Φ): RegexRule n α Φ :=
+def Rule.toRegex {n: Nat} {φ: Type}
+  (r: Rule n φ): RegexRule n φ :=
   (Regex.concat
     (Regex.symbol (Sum.inl r.enter))
     (Regex.concat
@@ -28,14 +27,14 @@ def Rule.toRegex {n: Nat} {α: Type} {Φ: (α: Type) -> Type}
     )
   )
 
-abbrev Rules (n: Nat) (α: Type) (Φ: (α: Type) -> Type) := { xs: List (Rule n α Φ) // xs.length > 0 }
+abbrev Rules (n: Nat) (φ: Type) := { xs: List (Rule n φ) // xs.length > 0 }
 
-structure BCFG (n: Nat) (α: Type) (Φ: (α: Type) -> Type) where
+structure BCFG (n: Nat) (φ: Type) where
   start: { s: List (Ref n) // s.length > 0 }
-  prods: Vec (Rules n α Φ) n
+  prods: Vec (Rules n φ) n
 
-def union_rules {n: Nat} {α: Type} {Φ: (α: Type) -> Type}
-  (xs: Rules n α Φ): RegexRule n α Φ :=
+def union_rules {n: Nat} {φ: Type}
+  (xs: Rules n φ): RegexRule n φ :=
   match xs with
   | Subtype.mk xs hxs =>
   match xs with
@@ -44,8 +43,8 @@ def union_rules {n: Nat} {α: Type} {Φ: (α: Type) -> Type}
   | (x::xs) => List.foldl Regex.or x.toRegex (List.map Rule.toRegex xs)
 
 def BCFG.getStart
-  {n: Nat} {α: Type} {Φ: (α: Type) -> Type}
-  (g: BCFG n α Φ): RegexRule n α Φ :=
+  {n: Nat} {φ: Type}
+  (g: BCFG n φ): RegexRule n φ :=
   match g.start with
   | Subtype.mk s hs =>
   match s with
@@ -54,32 +53,33 @@ def BCFG.getStart
     let xs' := (List.map (fun x' => Regex.symbol (Sum.inr x'))) xs
     List.foldl Regex.or (Regex.symbol (Sum.inr x)) xs'
 
-def BCFG.lookup {n: Nat} {α: Type} {Φ: (α: Type) -> Type}
-  (g: BCFG n α Φ) (ref: Fin n): RegexRule n α Φ :=
+def BCFG.lookup {n: Nat} {φ: Type}
+  (g: BCFG n φ) (ref: Fin n): RegexRule n φ :=
   union_rules (Vec.get g.prods ref)
 
-def nullable {n: Nat} {α: Type} {Φ: (α: Type) -> Type} (r: RegexRule n α Φ): Bool :=
+def nullable {n: Nat} {φ: Type} (r: RegexRule n φ): Bool :=
   Regex.nullable r
 
-partial def derive {n: Nat} {α: Type} [DecidableEq α] [BEq α]
-  (g: BCFG n α Pred) (r: RegexRule n α Pred) (a: α): RegexRule n α Pred :=
+partial def derive {n: Nat}
+  (g: BCFG n φ) (Φ: φ -> α -> Prop) [DecidableRel Φ]
+  (r: RegexRule n φ) (a: α): RegexRule n φ :=
   match r with
   | Regex.emptyset => Regex.emptyset
   | Regex.emptystr => Regex.emptyset
   | Regex.symbol (Sum.inl p) =>
-    if Pred.eval p a
+    if Φ p a
     then Regex.emptystr
     else Regex.emptyset
   | Regex.symbol (Sum.inr ref) =>
-    derive g (g.lookup ref) a
+    derive g Φ (g.lookup ref) a
   | Regex.or r1 r2 =>
-    Regex.or (derive g r1 a) (derive g r2 a)
+    Regex.or (derive g Φ r1 a) (derive g Φ r2 a)
   | Regex.concat r1 r2 =>
     if nullable r1
     then Regex.or
-      (Regex.concat (derive g r1 a) r2)
-      (derive g r2 a)
+      (Regex.concat (derive g Φ r1 a) r2)
+      (derive g Φ r2 a)
     else
-      (Regex.concat (derive g r1 a) r2)
+      (Regex.concat (derive g Φ r1 a) r2)
   | Regex.star r1 =>
-    Regex.concat (derive g r1 a) (Regex.star r1)
+    Regex.concat (derive g Φ r1 a) (Regex.star r1)
