Validator/Expr/Grammar99.lean
@@ -16,21 +16,23 @@ import Validator.Expr.Language
 --         n → a <r>, where n is a non-terminal in N, a is a symbol in Σ, and r is a regular expression comprising non-terminals,
 --     rf is a regular expression comprising non-terminals.
 
-structure Grammar99 (n: Nat) (α: Type) (Φ: (α: Type) -> Type) where
+structure Grammar99 (n: Nat) (φ: Type) where
   start: Regex (Ref n)
-  prods: Vec (Φ α × Regex (Ref n)) n
+  prods: Vec (φ × Regex (Ref n)) n
 
-def Grammar99.lookup (g: Grammar99 n α Φ) (ref: Fin n): Φ α × Regex (Ref n) :=
+def Grammar99.lookup (g: Grammar99 n φ) (ref: Fin n): φ × Regex (Ref n) :=
   Vec.get g.prods ref
 
-def Grammar99.denote_prod {α: Type} [BEq α] (g: Grammar99 n α Pred) (pred: Pred α) (r: Regex (Ref n)) (xs: Hedge α): Prop :=
+def Grammar99.denote_prod {α: Type}
+  (g: Grammar99 n φ) (Φ: φ -> α -> Prop) [DecidableRel Φ]
+  (pred: φ) (r: Regex (Ref n)) (xs: Hedge α): Prop :=
   match xs with
   | [Hedge.Node.mk label children] =>
-    Pred.eval pred label /\
+    Φ pred label /\
     Regex.denote_infix r children (fun ref xs' =>
       match (g.lookup ref) with
       | (pred', r') =>
-        Grammar99.denote_prod g pred' r' xs'
+        Grammar99.denote_prod g Φ pred' r' xs'
     )
   | _ => False
   termination_by xs
@@ -41,19 +43,25 @@ def Grammar99.denote_prod {α: Type} [BEq α] (g: Grammar99 n α Pred) (pred: Pr
     simp only [List.cons.sizeOf_spec, List.nil.sizeOf_spec, Hedge.Node.mk.sizeOf_spec]
     omega
 
-def Grammar99.denote_start {α: Type} [BEq α] (g: Grammar99 n α Pred) (r: Regex (Ref n)) (xs: Hedge α): Prop :=
+def Grammar99.denote_start {α: Type}
+  (g: Grammar99 n φ) (Φ: φ -> α -> Prop) [DecidableRel Φ]
+  (r: Regex (Ref n)) (xs: Hedge α): Prop :=
   Regex.denote_infix r xs (fun ref xs' =>
     match (g.lookup ref) with
     | (pred', r') =>
-      Grammar99.denote_prod g pred' r' xs'
+      Grammar99.denote_prod g Φ pred' r' xs'
   )
 
-def Grammar99.denote {α: Type} [BEq α] (g: Grammar99 n α Pred) (xs: Hedge α): Prop :=
-  Grammar99.denote_start g g.start xs
+def Grammar99.denote {α: Type}
+  (g: Grammar99 n φ) (Φ: φ -> α -> Prop) [DecidableRel Φ]
+  (xs: Hedge α): Prop :=
+  Grammar99.denote_start g Φ g.start xs
 
 namespace Grammar99
 
-def convert99' (g99: Grammar99 n α Φ) (r: Regex (Ref n)): Rule n α Φ :=
+def convert99'
+  (g99: Grammar99 n φ)
+  (r: Regex (Ref n)): Rule n φ :=
   match r with
   | Regex.emptyset => Regex.emptyset
   | Regex.emptystr => Regex.emptystr
@@ -62,12 +70,12 @@ def convert99' (g99: Grammar99 n α Φ) (r: Regex (Ref n)): Rule n α Φ :=
   | Regex.concat p q => Regex.concat (convert99' g99 p) (convert99' g99 q)
   | Regex.star p => Regex.star (convert99' g99 p)
 
-def convert99 (g99: Grammar99 n α Φ): Grammar n α Φ :=
+def convert99 (g99: Grammar99 n φ): Grammar n φ :=
   match g99 with
   | Grammar99.mk start prods =>
-    Grammar.mk (convert99' g99 start) (Vec.map (fun (_, rref) => convert99' g99 rref) prods)
+    Grammar.mk (convert99' g99 start) (Vec.map prods (fun (_, rref) => convert99' g99 rref))
 
-def convert' (g: Grammar n α Φ) (r: Regex (Φ α × Ref n)): Regex (Ref n) :=
+def convert' (g: Grammar n φ) (r: Regex (φ × Ref n)): Regex (Ref n) :=
   match r with
   | Regex.emptyset => Regex.emptyset
   | Regex.emptystr => Regex.emptystr
