Validator/Expr/IfExpr.lean
@@ -1,27 +1,31 @@
 import Validator.Std.Vec
 
-import Validator.Expr.Pred
 import Validator.Expr.Regex
 import Validator.Expr.Grammar
 
-inductive IfExpr n α where
-  | mk (cnd: Pred α) (thn: Fin n)
+abbrev IfExpr n φ := (φ × Fin n)
 
-abbrev IfExprs n α l := Vec (IfExpr n α) l
+abbrev IfExprs n φ l := Vec (IfExpr n φ) l
 
 namespace IfExpr
 
-def eval {α: Type} [DecidableEq α] (g: Grammar n (Pred α)) (ifExpr: IfExpr n α) (t: α): Rule n (Pred α) :=
+def eval {α: Type}
+  (g: Grammar n φ) (Φ: φ -> α -> Prop) [DecidableRel Φ]
+  (ifExpr: IfExpr n φ) (t: α): Rule n φ :=
   match ifExpr with
-  | IfExpr.mk cnd thn =>
-    if Pred.eval cnd t
+  | (cnd, thn) =>
+    if Φ cnd t
     then g.lookup thn
     else Regex.emptyset
 
-def evals {α: Type} {n: Nat} [DecidableEq α] (g: Grammar n (Pred α)) (ifExprs: IfExprs n α l) (t: α): Rules n (Pred α) l :=
-  Vec.map ifExprs (fun x => eval g x t)
+def evals {α: Type} {n: Nat}
+  (g: Grammar n φ) (Φ: φ -> α -> Prop) [DecidableRel Φ]
+  (ifExprs: IfExprs n φ l) (t: α): Rules n φ l :=
+  Vec.map ifExprs (fun x => eval g Φ x t)
 
-theorem evals_nil_is_nil {α: Type} {n: Nat} [DecidableEq α] (g: Grammar n (Pred α)) (a: α):
-  evals g (n := n) Vec.nil a = Vec.nil := by
+theorem evals_nil_is_nil {α: Type} {n: Nat}
+  (g: Grammar n φ) (Φ: φ -> α -> Prop) [DecidableRel Φ]
+  (a: α):
+  evals g Φ (n := n) Vec.nil a = Vec.nil := by
   unfold evals
   simp only [Vec.map_nil]
