Validator/Learning/Original.lean
@@ -16,7 +16,7 @@ namespace Original
 -- foldLoop is a more readable version of List.foldl for imperative programmers:
 -- Imperative programmers can imagine that `Id (Expr α)` = `Expr α`, because it does.
 -- The Id wrapper just adds a monad wrapper to enable the do notation, so that we can use the for loop in Lean.
-private def foldLoop (deriv: Rule n (Pred α) -> Hedge.Node α -> Rule n (Pred α)) (start: Rule n (Pred α)) (hedge: Hedge α): Id (Rule n (Pred α)) := do
+private def foldLoop (deriv: Rule n φ -> Hedge.Node α -> Rule n φ) (start: Rule n φ) (hedge: Hedge α): Id (Rule n φ) := do
   let mut res := start
   for tree in hedge do
     res := deriv res tree
@@ -26,31 +26,35 @@ private def foldLoop (deriv: Rule n (Pred α) -> Hedge.Node α -> Rule n (Pred �
 -- It returns the expression that is left to match after matching the tree.
 -- Note we need to use `partial`, since Lean cannot automatically figure out that the derive function terminates.
 -- In OriginalTotal we show how to remove this, by manually proving that it in fact does terminate.
-partial def derive [DecidableEq α] (g: Grammar n (Pred α)) (x: Rule n (Pred α)) (tree: Hedge.Node α): Rule n (Pred α) :=
+partial def derive
+  (g: Grammar n φ) (Φ: φ -> α -> Prop) [DecidableRel Φ]
+  (x: Rule n φ) (tree: Hedge.Node α): Rule n φ :=
   match x with
   | Regex.emptyset => Regex.emptyset
   | Regex.emptystr => Regex.emptyset
   | Regex.symbol (labelPred, childRef) =>
     -- This is the only rule that differs from regular expressions.
     -- Although if we view this as a complicated predicate, then actually there is no difference.
-    if Pred.eval labelPred (Hedge.Node.getLabel tree)
+    if Φ labelPred (Hedge.Node.getLabel tree)
     -- This is exactly the same as: validate childrenExpr (Hedge.Node.getChildren tree)
-    && Regex.nullable (List.foldl (derive g) (g.lookup childRef) (Hedge.Node.getChildren tree))
+    && Regex.nullable (List.foldl (derive g Φ) (g.lookup childRef) (Hedge.Node.getChildren tree))
     -- Just like with char, if the predicate matches we return emptystr and if it doesn't we return emptyset
     then Regex.emptystr
     else Regex.emptyset
-  | Regex.or y z => Regex.or (derive g y tree) (derive g z tree)
+  | Regex.or y z => Regex.or (derive g Φ y tree) (derive g Φ z tree)
   | Regex.concat y z =>
     if Regex.nullable y
-    then Regex.or (Regex.concat (derive g y tree) z) (derive g z tree)
-    else Regex.concat (derive g y tree) z
-  | Regex.star y => Regex.concat (derive g y tree) (Regex.star y)
+    then Regex.or (Regex.concat (derive g Φ y tree) z) (derive g Φ z tree)
+    else Regex.concat (derive g Φ y tree) z
+  | Regex.star y => Regex.concat (derive g Φ y tree) (Regex.star y)
 
-partial def validate [DecidableEq α] (g: Grammar n (Pred α)) (x: Rule n (Pred α)) (hedge: Hedge α): Bool :=
-  Rule.nullable (List.foldl (derive g) x hedge)
+partial def validate
+  (g: Grammar n φ) (Φ: φ -> α -> Prop) [DecidableRel Φ]
+  (x: Rule n φ) (hedge: Hedge α): Bool :=
+  Rule.nullable (List.foldl (derive g Φ) x hedge)
 
 def run [DecidableEq α] (g: Grammar n (Pred α)) (t: Hedge.Node α): Except String Bool :=
-  Except.ok (validate g g.start [t])
+  Except.ok (validate g Pred.eval g.start [t])
 
 -- Tests
 
