Validator/Learning/Parser.lean
@@ -22,44 +22,52 @@ import Validator.Validator.Inst.TreeParserM
 
 namespace Parser
 
-def deriveEnter [DecidableEq α] [ValidateM m n α] (g: Grammar n (Pred α)) (xs: Rules n (Pred α) l): m (Rules n (Pred α) (Symbol.nums xs)) := do
+def deriveEnter [DecidableEq φ] [ValidateM m n φ α]
+  (g: Grammar n φ) (Φ: φ -> α -> Prop) [DecidableRel Φ]
+  (xs: Rules n φ l): m (Rules n φ (Symbol.nums xs)) := do
   let enters <- Enter.DeriveEnter.deriveEnter xs
   let token <- Parser.token
-  return IfExpr.evals g enters token
+  return IfExpr.evals g Φ enters token
 
-def deriveLeaveM [DecidableEq α] [ValidateM m n α] (xs: Rules n (Pred α) l) (cs: Rules n (Pred α) (Symbol.nums xs)): m (Rules n (Pred α) l) :=
+def deriveLeaveM [DecidableEq φ] [ValidateM m n φ α] (xs: Rules n φ l) (cs: Rules n φ (Symbol.nums xs)): m (Rules n φ l) :=
   Leave.DeriveLeaveM.deriveLeaveM xs (Vec.map cs Rule.nullable)
 
-def deriveValue [DecidableEq α] [ValidateM m n α] (g: Grammar n (Pred α)) (xs: Rules n (Pred α) l): m (Rules n (Pred α) l) := do
-  deriveEnter g xs >>= deriveLeaveM xs
+def deriveValue [DecidableEq φ] [ValidateM m n φ α]
+  (g: Grammar n φ) (Φ: φ -> α -> Prop) [DecidableRel Φ]
+  (xs: Rules n φ l): m (Rules n φ l) := do
+  deriveEnter g Φ xs >>= deriveLeaveM (α := α) xs
 
 -- TODO: Is it possible to have a Parser type that can be proved to be of the correct shape, and have not expection throwing
 -- for example: can you prove that your Parser will never return an Hint.leave after returning a Hint.field.
 -- This class can be called the LawfulParser.
-partial def derive [DecidableEq α] [ValidateM m n α] (g: Grammar n (Pred α)) (xs: Rules n (Pred α) l): m (Rules n (Pred α) l) := do
+partial def derive [DecidableEq φ] [ValidateM m n φ α]
+  (g: Grammar n φ) (Φ: φ -> α -> Prop) [DecidableRel Φ]
+  (xs: Rules n φ l): m (Rules n φ l) := do
   if List.all xs.toList Regex.unescapable then
     Parser.skip; return xs
   match <- Parser.next with
   | Hint.field =>
-    let childxs <- deriveEnter g xs -- derive enter field
+    let childxs <- deriveEnter g Φ xs -- derive enter field
     let dchildxs <-
       match <- Parser.next with
-      | Hint.value => deriveValue g childxs -- derive child value
-      | Hint.enter => derive g childxs -- derive children, until return from a Hint.leave
+      | Hint.value => deriveValue g Φ childxs -- derive child value
+      | Hint.enter => derive g Φ childxs -- derive children, until return from a Hint.leave
       | hint => throw s!"unexpected {hint}"
-    let xsLeave <- deriveLeaveM xs dchildxs -- derive leave field
-    derive g xsLeave -- deriv next
-  | Hint.value => deriveValue g xs >>= derive g -- derive value and then derive next
-  | Hint.enter => derive g xs >>= derive g -- derive children, until return from a Hint.leave and then derive next
+    let xsLeave <- deriveLeaveM (α := α) xs dchildxs -- derive leave field
+    derive g Φ xsLeave -- deriv next
+  | Hint.value => deriveValue g Φ xs >>= derive g Φ -- derive value and then derive next
+  | Hint.enter => derive g Φ xs >>= derive g Φ -- derive children, until return from a Hint.leave and then derive next
   | Hint.leave => return xs -- never happens at the top
   | Hint.eof => return xs -- only happens at the top
 
-def validate {m} [DecidableEq α] [ValidateM m n α] (g: Grammar n (Pred α)) (x: Rule n (Pred α)): m Bool := do
-  let dxs <- derive g (Vec.cons x Vec.nil)
+def validate {m} [DecidableEq φ] [ValidateM m n φ α]
+  (g: Grammar n φ) (Φ: φ -> α -> Prop) [DecidableRel Φ]
+  (x: Rule n φ): m Bool := do
+  let dxs <- derive g Φ (Vec.cons x Vec.nil)
   return Rule.nullable dxs.head
 
 def run [DecidableEq α] (g: Grammar n (Pred α)) (t: Hedge.Node α): Except String Bool :=
-  TreeParserM.run' (validate g g.start) t
+  TreeParserM.run' (validate g Pred.eval g.start) t
 
 -- Tests
 
