Validator/Derive/Enter.lean
@@ -7,10 +7,8 @@ import Validator.Expr.Symbol
 
 namespace Enter
 
-def deriveEnter (xs: Rules n (Pred α) l): IfExprs n α (Symbol.nums xs) :=
-  Vec.map
-    (Symbol.extractsFrom xs).2
-    (fun (pred, ref) => IfExpr.mk pred ref)
+def deriveEnter (xs: Rules n φ l): IfExprs n φ (Symbol.nums xs) :=
+  (Symbol.extractsFrom xs).2
 
-class DeriveEnter (m: Type -> Type u) (n: Nat) (α: outParam Type) where
-  deriveEnter {l: Nat} (xs: Rules n (Pred α) l): m (IfExprs n α (Symbol.nums xs))
+class DeriveEnter (m: Type -> Type u) (n: Nat) (φ: Type) where
+  deriveEnter {l: Nat} (xs: Rules n φ l): m (IfExprs n φ (Symbol.nums xs))
