Validator/Derive/Leave.lean
@@ -11,16 +11,16 @@ namespace Leave
 -- The vectors of bools represent the nullability of the derived child expressions.
 -- Each bool will then replace each symbol expression with either an emptystr or emptyset.
 def deriveLeaves
-  (xs: Rules n (Pred α) l)
+  (xs: Rules n φ l)
   (ns: Vec Bool (Symbol.nums xs))
-  : (Rules n (Pred α) l) :=
+  : (Rules n φ l) :=
   let (regexes, symbols) := Symbol.extractsFrom xs
-  let res: Vec ((Pred α × Ref n) × Bool) (Symbol.nums xs) := Vec.zip symbols ns
-  let res': Vec (Regex ((Pred α × Ref n) × Bool)) l := Symbol.replacesFrom regexes res
+  let res: Vec ((φ × Ref n) × Bool) (Symbol.nums xs) := Vec.zip symbols ns
+  let res': Vec (Regex ((φ × Ref n) × Bool)) l := Symbol.replacesFrom regexes res
   Regex.smartDerives2 res'
 
-def deriveLeaveM [Monad m] {n: Nat} {l: Nat} (xs: Rules n (Pred α) l) (ns: Vec Bool (Symbol.nums xs)): m (Rules n (Pred α) l) := do
+def deriveLeaveM [Monad m] {n: Nat} {l: Nat} (xs: Rules n φ l) (ns: Vec Bool (Symbol.nums xs)): m (Rules n φ l) := do
   return deriveLeaves xs ns
 
-class DeriveLeaveM (m: Type -> Type u) (n: Nat) (α: outParam Type) where
-  deriveLeaveM {l: Nat} (xs: Rules n (Pred α) l) (ns: Vec Bool (Symbol.nums xs)): m (Rules n (Pred α) l)
+class DeriveLeaveM (m: Type -> Type u) (n: Nat) (φ: Type) where
+  deriveLeaveM {l: Nat} (xs: Rules n φ l) (ns: Vec Bool (Symbol.nums xs)): m (Rules n φ l)
